@prefix odrl: <http://www.w3.org/ns/odrl/2/> .
@prefix rdf: <http://www.w3.org/1999/02/22-rdf-syntax-ns#> .
@prefix rdfs: <http://www.w3.org/2000/01/rdf-schema#> .
@prefix skos: <http://www.w3.org/2004/02/skos/core#> .
@prefix owl: <http://www.w3.org/2002/07/owl#> .
@prefix xsd: <http://www.w3.org/2001/XMLSchema#> .
@prefix dct: <http://purl.org/dc/terms/> .
@prefix schema: <http://schema.org/> .
@prefix foaf: <http://xmlns.com/foaf/0.1/> .
@prefix vcard: <http://www.w3.org/2006/vcard/ns#> .
@prefix cc: <http://creativecommons.org/ns#> .

@prefix ods: <https://w3id.org/ods/> .

ods:
	a owl:Ontology ;
	rdfs:label "ODRL Profile for Data Sovereignty"@en ;
	owl:versionInfo "0.1" ;
	dct:creator "Arghavan Hosseinzadeh", "Robin Brandstaedter", "Jessica Chwalek";
	dcterms:publisher "Fraunhofer IESE" ;
	dct:description "Data sovereignty is a key success factor for data-driven business models and has the goal of providing Data Providers with full control over their data. The ODRL Profile for Data Sovereignty specifies the terms to express usage restrictions, obligations and modifications."@en ;
	rdfs:comment "This is the RDF ontology for the ODRL Profile for Data Sovereignty."@en ;
	dcterms:bibliographicCitation "Cite this vocabulary as: Hosseinzadeh, A., Brandstaedter, R., & Chwalek, J. (2024). ODRL Profile for Data Sovereignty 0.1. https:// "@en ;
	vann:preferredNamespacePrefix "ods" ;
	vann:preferredNamespaceUri "https://w3id.org/ods#"^^xsd:string ;
	dcterms:created "2023-03-13"^^xsd:date ;
	dcterms:modified "2024-05-14"^^xsd:date ;
	foaf:logo <https://github.com/Fraunhofer-IESE/ODS/blob/main/ODS-128.png> ;
	dct:license <https://www.apache.org/licenses/LICENSE-2.0.txt> .

## SKOS Collections for Grouping related concepts.
## ODRL Vocabulary

<http://www.w3.org/ns/odrl/2/#constraintLogicalOperands>
    a skos:Collection ;
    skos:prefLabel "Logical Constraint Operands"@en ;
    skos:scopeNote "ODRL Core Vocabulary Terms"@en ;
    skos:member :or ;
    skos:member :xone ;
    skos:member :and ;
    skos:member :andSequence .

<http://www.w3.org/ns/odrl/2/#constraintRelationalOperators>
    a skos:Collection ;
    skos:prefLabel "Constraint Operators"@en ;
    skos:scopeNote "ODRL Core Vocabulary Terms"@en ;
    skos:member :eq ;
    skos:member :gt ;
    skos:member :gteq ;
    skos:member :lt ;
    skos:member :lteq ;
    skos:member :neq ;
    skos:member :isA ;
    skos:member :hasPart ;
    skos:member :isPartOf ;
    skos:member :isAllOf ;
    skos:member :isAnyOf ;
    skos:member :isNoneOf .

<http://www.w3.org/ns/odrl/2/#actions>
    a skos:Collection ;
    skos:prefLabel "Actions for Rules"@en ;
    skos:scopeNote "ODRL Core Vocabulary Terms"@en ;
    skos:member :use ;
    skos:member :transfer .

<http://www.w3.org/ns/odrl/2/#actionsCommon>
    a skos:Collection ;
    skos:prefLabel "Actions for Rules"@en ;
    skos:scopeNote "ODRL Common Vocabulary Terms"@en ;
    skos:member :acceptTracking ;
    skos:member :aggregate ;
    skos:member :annotate ;
    skos:member :anonymize ;
    skos:member :archive ;
    skos:member :attribute ;
    skos:member cc:Attribution ;
    skos:member cc:CommercialUse ;
    skos:member :compensate ;
    skos:member :concurrentUse ;
    skos:member :delete ;
    skos:member :derive ;
    skos:member cc:DerivativeWorks ;
    skos:member :digitize ;
    skos:member :display ;
    skos:member :distribute ;
    skos:member cc:Distribution ;
    skos:member :ensureExclusivity ;
    skos:member :execute ;
    skos:member :extract ;
    skos:member :give ;
    skos:member :grantUse ;
    skos:member :include ;
    skos:member :index ;
    skos:member :inform ;
    skos:member :install ;
    skos:member :modify ;
    skos:member :move ;
    skos:member :nextPolicy ;
    skos:member cc:Notice ;
    skos:member :obtainConsent ;
    skos:member :play ;
    skos:member :present ;
    skos:member :print ;
    skos:member :read ;
    skos:member :reproduce ;
    skos:member cc:Reproduction ;
    skos:member :reviewPolicy ;
    skos:member :sell ;
    skos:member cc:ShareAlike ;
    skos:member cc:Sharing ;
    skos:member cc:SourceCode ;
    skos:member :stream ;
    skos:member :synchronize ;
    skos:member :textToSpeech ;
    skos:member :transform ;
    skos:member :translate ;
    skos:member :uninstall ;
    skos:member :watermark .

<http://www.w3.org/ns/odrl/2/#constraintLeftOperandCommon>
    a skos:Collection ;
    skos:prefLabel "Constraint Left Operands"@en ;
    skos:scopeNote "ODRL Common Vocabulary Terms"@en ;
    skos:member :absolutePosition ;
    skos:member :absoluteSpatialPosition ;
    skos:member :absoluteTemporalPosition ;
    skos:member :absoluteSize ;
    skos:member :count ;
    skos:member :dateTime ;
    skos:member :delayPeriod ;
    skos:member :deliveryChannel ;
    skos:member :elapsedTime ;
    skos:member :event ;
    skos:member :fileFormat ;
    skos:member :industry ;
    skos:member :language ;
    skos:member :media ;
    skos:member :meteredTime ;
    skos:member :payAmount ;
    skos:member :percentage ;
    skos:member :product ;
    skos:member :purpose ;
    skos:member :recipient ;
    skos:member :relativePosition ;
    skos:member :relativeSpatialPosition ;
    skos:member :relativeTemporalPosition ;
    skos:member :relativeSize ;
    skos:member :resolution ;
    skos:member :spatial ;
    skos:member :spatialCoordinates ;
    skos:member :systemDevice ;
    skos:member :timeInterval ;
    skos:member :unitOfCount ;
    skos:member :version ;
    skos:member :virtualLocation .

<http://www.w3.org/ns/odrl/2/#constraintRightOpCommon>
	a skos:Collection ;
	skos:prefLabel "Constraint Right Operands"@en ;
	skos:scopeNote "ODRL Common Vocabulary Terms"@en ;
	skos:member :policyUsage .

## SKOS Collections for Grouping related concepts.
## ods Vocabulary

<https://w3id.org/ods/#data-usage-control-concepts>
    a skos:Collection ;
    skos:prefLabel "Usage Control Component"@en ;
    skos:scopeNote "oac Vocabulary Terms"@en ;
    skos:member :UsageControlComponent ;
	skos:member :hasPIP ;
	skos:member :hasPXP ;
    skos:member :interfaceDescription ;
    skos:member :endpointURI .

<https://w3id.org/ods/#constraint-operators>
	a skos:Collection ;
	skos:prefLabel "Constraint Operators"@en ;
	skos:scopeNote "oac Vocabulary Terms"@en ;
	# Set operator
	skos:member ods:in ;
	skos:member ods:subset .

<https://w3id.org/ods/#actions-for-rules>
    a skos:Collection ;
    skos:prefLabel "Actions for Rules"@en ;
    skos:scopeNote "ods Vocabulary Terms"@en ;
    skos:member ods:add ;
    skos:member ods:divide ;
    skos:member ods:encrypt ;
    skos:member ods:hash ;
    skos:member ods:log ;
    skos:member ods:multiply ;
    skos:member ods:mpc ;
    skos:member ods:notify ;
    skos:member ods:query ;
    skos:member ods:replace ;
    skos:member ods:shuffle .

<https://w3id.org/ods/#constraint-left-operands>
    a skos:Collection ;
    skos:prefLabel "Constraint Left Operands"@en ;
    skos:scopeNote "ods Vocabulary Terms"@en ;
    skos:member ods:application ;
    skos:member ods:artifactState ;
    skos:member ods:endpoint ;
    skos:member ods:function ;
    skos:member ods:hashAlgorithm ;
    skos:member ods:encryptionAlgorithm ;
    skos:member ods:jsonPath ;
    skos:member ods:jsonStringPath ;
    skos:member ods:logLevel ;
    skos:member ods:notificationLevel ;
    skos:member ods:operand ;
    skos:member ods:path ;
    skos:member ods:quantity ;
    skos:member ods:replaceWith ;
    skos:member ods:role ;
    skos:member ods:state ;
    skos:member ods:user ;
    skos:member ods:xPath ;


<https://w3id.org/ods/#constraint-right-operands>
	a skos:Collection ;
    skos:prefLabel "Constraint Right Operands"@en ;
    skos:scopeNote "ods Vocabulary Terms"@en ;
	# values for Artifact State
	skos:member ods:anonymized ;
	skos:member ods:combined  ;
	skos:member ods:encrypted  ;
	skos:member ods:pseudonymized  ;
	# values for Log and Notification Level
	skos:member ods:onActionOperated   ;
	skos:member ods:onAllow   ;
	skos:member ods:onDeny   ;
	skos:member ods:onDutyExercised   ;
	# values for Function
	skos:member ods:maximum ;
	skos:member ods:minimum ;
	skos:member ods:sum .

## ODRL Profile for Data Sovereignty
## Data Usage Control concepts

:UsageControlComponent
	a rdfs:Class, owl:Class, skos:Concept ;
	rdfs:isDefinedBy ods: ;
	skos:definition "It refers to data usage control components."@en ;
	skos:note "It is optional to explicitly specify a data usage control component that is responsible for providing context information or executing a duty action."@en ;
	rdfs:label "Usage Control Component"@en .

:hasPIP
	a rdf:Property , owl:ObjectProperty, skos:Concept ;
	rdfs:isDefinedBy ods: ;
	rdfs:label "has Policy Information Point"@en ;
	skos:definition "A Usage Control Component that provides needed information for evaluating a constraint."@en ;
	rdfs:domain :Constraint ;
	rdfs:range :UsageControlComponent  .

:hasPXP
	a rdf:Property , owl:ObjectProperty, skos:Concept ;
	rdfs:isDefinedBy ods: ;
	rdfs:label "has Policy Execution Point"@en ;
	skos:definition "A Usage Control Component that executes an action."@en ;
	rdfs:domain :Action ;
	rdfs:range :UsageControlComponent  .

:interfaceDescription
	a rdf:Property , owl:ObjectProperty, skos:Concept ;
	rdfs:isDefinedBy ods: ;
	rdfs:label "Interface Description"@en ;
	skos:definition "The reference to a URI that provides the interface description of a usage control endpoint."@en ;
	rdfs:domain :UsageControlComponent ;
	rdfs:range :UsageControlComponent  .

:endpointURI
	a rdf:Property , owl:ObjectProperty, skos:Concept ;
	rdfs:isDefinedBy ods: ;
	rdfs:label "Endpoint URI"@en ;
	skos:definition "The reference to a URI that expresses an exact endpoint of that usage control endpoint."@en ;
	rdfs:domain :UsageControlComponent ;
	rdfs:range :UsageControlComponent  .

## ods Operators

ods:in
	a :Operator, owl:NamedIndividual, skos:Concept ;
	rdfs:isDefinedBy ods: ;
	rdfs:label "In"@en ;
	skos:definition "This operator is used to express the membership of an individual element in a set."@en ;
	skos:scopeNote "Non-Normative"@en .

ods:subset
	a :Operator, owl:NamedIndividual, skos:Concept ;
	rdfs:isDefinedBy ods: ;
	rdfs:label "Subset"@en ;
	skos:definition "This operator is used to indicate that one set is entirely contained within another set."@en ;
	skos:scopeNote "Non-Normative"@en .

## ods Actions

ods:add
	a :Action, skos:Concept ;
	rdfs:isDefinedBy ods: ;
	:includedIn odrl:use ;
	rdfs:label "Add"@en ;
	skos:definition "To modify a number by adding a given value to it."@en ;
	skos:note "The field to be modified can be specified using ods:jsonPath or ods:xPath and the given value can be specified using ods:operand."@en ;
	skos:scopeNote "Non-Normative"@en .

ods:divide
	a :Action, skos:Concept ;
	rdfs:isDefinedBy ods: ;
	:includedIn odrl:use ;
	rdfs:label "Divide"@en ;
	skos:definition "To modify a number by dividing it by a given value."@en ;
	skos:note "The field to be modified can be specified using ods:jsonPath or ods:xPath and the given value can be specified using ods:operand."@en ;
	skos:scopeNote "Non-Normative"@en .

ods:encrypt
	a :Action, skos:Concept ;
	rdfs:isDefinedBy ods: ;
	:includedIn odrl:use ;
	rdfs:label "Encrypt"@en ;
	skos:definition "To encrpyt a data artifact or parts of it to secure it during transmission and to prevent unauthorized access. The encryption algorithm might be specified by a constraint."@en ;
	skos:note "The encryption algorithm can be specified using ods:encryptionAlgorithm (eg. AES)."@en ;
	skos:scopeNote "Non-Normative"@en .

ods:hash
	a :Action, skos:Concept ;
	rdfs:isDefinedBy ods: ;
	:includedIn odrl:use ;
	rdfs:label "Hash"@en ;
	skos:definition "To modify a value by replacing it with a hash of the value."@en ;
	skos:note "The field to be modified can be specified using ods:jsonPath or ods:xPath and the hash algorithm can be specified using ods:hashAlgorithm (eg. SHA256)."@en ;
	skos:scopeNote "Non-Normative"@en .

ods:log
	a :Action, skos:Concept ;
	rdfs:isDefinedBy ods: ;
	:includedIn odrl:use ;
	rdfs:label "Log"@en ;
	skos:definition "To log information about data usage. It is used to create transparency."@en ;
	skos:note "The log level can be specified using ods:logLevel left operand."@en ;
	skos:scopeNote "Non-Normative"@en .

ods:multiply
	a :Action, skos:Concept ;
	rdfs:isDefinedBy ods: ;
	:includedIn odrl:use ;
	rdfs:label "Multiply"@en ;
	skos:definition "To modify a number by multiplying it to a given value."@en ;
	skos:note "The field to be modified can be specified using ods:jsonPath or ods:xPath and the given value can be specified using ods:operand."@en ;
	skos:scopeNote "Non-Normative"@en .

ods:mpc
	a :Action, skos:Concept ;
	rdfs:isDefinedBy ods: ;
	:includedIn odrl:use ;
	rdfs:label "Multiparty Computation"@en ;
	skos:definition "Secure Multiparty Computation (MPC) is a cryptographic protocol that enables a defined set of parties, each party owning a secret value, to compute a function collaboratively while preserving the privacy of their individual inputs."@en ;
	skos:scopeNote "Non-Normative"@en .

ods:notify
	a :Action, skos:Concept ;
	rdfs:isDefinedBy ods: ;
	:includedIn odrl:use ;
	rdfs:label "Notify"@en ;
	skos:definition "To notify a party with information about data usage."@en ;
	skos:note "The notification level can be specified using ods:notificationLevel left operand."@en ;
	skos:scopeNote "Non-Normative"@en .

ods:query
	a :Action, skos:Concept ;
	rdfs:isDefinedBy ods: ;
	:includedIn odrl:use ;
	rdfs:label "Query"@en ;
	skos:definition "To request for a piece of information or data from an information system or a database."@en ;
	skos:scopeNote "Non-Normative"@en .

ods:replace
	a :Action, skos:Concept ;
	rdfs:isDefinedBy ods: ;
	:includedIn odrl:use ;
	rdfs:label "Replace"@en ;
	skos:definition "To replace a field by a given value."@en ;
	skos:note "The field to be modified can be specified using ods:jsonPath or ods:xPath and the given value can be specified using ods:replaceWith."@en ;
	skos:scopeNote "Non-Normative"@en .

ods:shuffle
	a :Action, skos:Concept ;
	rdfs:isDefinedBy ods: ;
	:includedIn odrl:use ;
	rdfs:label "Shuffle"@en ;
	skos:definition "To replace a field with an anagram of it's value."@en ;
	skos:note "The field to be modified can be specified using ods:jsonPath or ods:xPath."@en ;
	skos:scopeNote "Non-Normative"@en .


## ods Left Operands

ods:application
	a :LeftOperand, owl:NamedIndividual, skos:Concept ;
	rdfs:isDefinedBy ods: ;
	rdfs:label "Application"@en ;
	skos:definition "An application is a program or piece of software designed to fulfill a particular purpose."@en ;
    skos:scopeNote "Non-Normative"@en .

ods:artifactState
	a :LeftOperand, owl:NamedIndividual, skos:Concept ;
	rdfs:isDefinedBy ods: ;
	rdfs:label "Artifact State"@en ;
	skos:definition "It refers to the status of a data asset."@en ;
	skos:note "This operand accepts the following values: ods:anonymized, ods:combined, ods:encrypted, ods:pseudonymized."@en ;
    skos:scopeNote "Non-Normative"@en .

ods:endpoint
	a :LeftOperand, owl:NamedIndividual, skos:Concept ;
	rdfs:isDefinedBy ods: ;
	rdfs:label "Endpoint"@en ;
	skos:definition "An endpoint refers to a specific address or connection point."@en ;
    skos:scopeNote "Non-Normative"@en .

ods:function
	a :LeftOperand, owl:NamedIndividual, skos:Concept ;
	rdfs:isDefinedBy ods: ;
	rdfs:label "Function"@en ;
	skos:definition "A function encapsulates a reusable logic."@en ;
	skos:note "In mathematical contexts, examples include ods:maximum, ods:minimum, and ods:sum."@en ;
    skos:scopeNote "Non-Normative"@en .

ods:hashAlgorithm
	a :LeftOperand, owl:NamedIndividual, skos:Concept ;
	rdfs:isDefinedBy ods: ;
	rdfs:label "Hash Algorithm"@en ;
	skos:definition "It indicates the hash value to be used."@en ;
	skos:note "For example, SHA256."@en ;
    skos:scopeNote "Non-Normative"@en .

ods:encryptionAlgorithm
	a :LeftOperand, owl:NamedIndividual, skos:Concept ;
	rdfs:isDefinedBy ods: ;
	rdfs:label "Encryption Algorithm"@en ;
	skos:definition "It indicates the encryption algorithm to be used."@en ;
	skos:note "For example, AES."@en ;
    skos:scopeNote "Non-Normative"@en .

ods:jsonPath
	a :LeftOperand, owl:NamedIndividual, skos:Concept ;
	rdfs:isDefinedBy ods: ;
	rdfs:label "JSONPath"@en ;
	skos:definition "An expression that refers to a part of a JSON structured data."@en ;
    skos:scopeNote "Non-Normative"@en .

ods:jsonStringPath
	a :LeftOperand, owl:NamedIndividual, skos:Concept ;
	rdfs:isDefinedBy ods: ;
	rdfs:label "JSON String Path"@en ;
	skos:definition "An expression that refers to a part of a JSON structured data."@en ;
	skos:note "It is used by Rego policy language."@en ;
    skos:scopeNote "Non-Normative"@en .

ods:logLevel
	a :LeftOperand, owl:NamedIndividual, skos:Concept ;
	rdfs:isDefinedBy ods: ;
	rdfs:label "Log Level"@en ;
	skos:definition "It refers to the log level."@en ;
	skos:note "This operand accepts the following values: ods:onActionOperated, ods:onAllow, ods:onDeny, ods:onDutyExercised."@en ;
    skos:scopeNote "Non-Normative"@en .

ods:notificationLevel
	a :LeftOperand, owl:NamedIndividual, skos:Concept ;
	rdfs:isDefinedBy ods: ;
	rdfs:label "Notification Level"@en ;
	skos:definition "It refers to the notification level."@en ;
	skos:note "This operand accepts the following values: ods:onActionOperated, ods:onAllow, ods:onDeny, ods:onDutyExercised."@en ;
    skos:scopeNote "Non-Normative"@en .

ods:operand
	a :LeftOperand, owl:NamedIndividual, skos:Concept ;
	rdfs:isDefinedBy ods: ;
	rdfs:label "Operand"@en ;
	skos:definition "An operand is a required element within an arithmetic or logical operation."@en ;
	skos:note "Operands can be numeric values or expressions."@en ;
	skos:scopeNote "Non-Normative"@en .

ods:path
	a :LeftOperand, owl:NamedIndividual, skos:Concept ;
	rdfs:isDefinedBy ods: ;
	rdfs:label "Path"@en ;
	skos:definition "An expression that refers to a file within a system, or an element within a hierarchical structure."@en ;
	skos:scopeNote "Non-Normative"@en .

ods:replaceWith
	a :LeftOperand, owl:NamedIndividual, skos:Concept ;
	rdfs:isDefinedBy ods: ;
	rdfs:label "Replace With"@en ;
	skos:definition "It specifies a new value for a specific field."@en ;
	skos:note "It gives a value for ods:replace action."@en ;
    skos:scopeNote "Non-Normative"@en .

ods:role
	a :LeftOperand, owl:NamedIndividual, skos:Concept ;
	rdfs:isDefinedBy ods: ;
	rdfs:label "Role"@en ;
	skos:definition "Role refers to an end user's role."@en ;
    skos:scopeNote "Non-Normative"@en .

ods:state
	a :LeftOperand, owl:NamedIndividual, skos:Concept ;
	rdfs:isDefinedBy ods: ;
	rdfs:label "State"@en ;
	skos:definition "It refers to an environment state."@en ;
	skos:note "Not be confused with artifact state."@en ;
    skos:scopeNote "Non-Normative"@en .

ods:user
	a :LeftOperand, owl:NamedIndividual, skos:Concept ;
	rdfs:isDefinedBy ods: ;
	rdfs:label "User"@en ;
	skos:definition "It refers to a particular end user."@en ;
    skos:scopeNote "Non-Normative"@en .

ods:xPath
	a :LeftOperand, owl:NamedIndividual, skos:Concept ;
	rdfs:isDefinedBy ods: ;
	rdfs:label "xPath"@en ;
	skos:definition "An expression that refers to specific elements of an XML document."@en ;
    skos:scopeNote "Non-Normative"@en .


## ods Right Operands

ods:anonymized
	a :RightOperand, owl:NamedIndividual, skos:Concept ;
	rdfs:isDefinedBy ods: ;
	rdfs:label "Anonymized"@en ;
	skos:definition "Indicates that the asset is anonymized."@en ;
    skos:scopeNote "Non-Normative"@en .

ods:combined
	a :RightOperand, owl:NamedIndividual, skos:Concept ;
	rdfs:isDefinedBy ods: ;
	rdfs:label "Combined"@en ;
	skos:definition "Indicates that the asset is combined."@en ;
    skos:scopeNote "Non-Normative"@en .

ods:encrypted
	a :RightOperand, owl:NamedIndividual, skos:Concept ;
	rdfs:isDefinedBy ods: ;
	rdfs:label "Encrypted"@en ;
	skos:definition "Indicates that the asset is encrypted."@en ;
    skos:scopeNote "Non-Normative"@en .

ods:maximum
	a :RightOperand, owl:NamedIndividual, skos:Concept ;
	rdfs:isDefinedBy ods: ;
	rdfs:label "Maximum"@en ;
	skos:definition "The maximum function to determine the largest value among a set of numbers."@en ;
    skos:scopeNote "Non-Normative"@en .

ods:minimum
	a :RightOperand, owl:NamedIndividual, skos:Concept ;
	rdfs:isDefinedBy ods: ;
	rdfs:label "Minimum"@en ;
	skos:definition "The minimum function to determine the smallest value among a set of numbers."@en ;
    skos:scopeNote "Non-Normative"@en .

ods:onActionOperated
	a :RightOperand, owl:NamedIndividual, skos:Concept ;
	rdfs:isDefinedBy ods: ;
	rdfs:label "On action operated"@en ;
	skos:definition "Log usage information or notify a party when the action of the rule is operated."@en ;
    skos:scopeNote "Non-Normative"@en .

ods:onAllow 
	a :RightOperand, owl:NamedIndividual, skos:Concept ;
	rdfs:isDefinedBy ods: ;
	rdfs:label "On allow"@en ;
	skos:definition "Log usage information or notify a party when performing the action of the rule is permitted."@en ;
    skos:scopeNote "Non-Normative"@en .

ods:onDeny
	a :RightOperand, owl:NamedIndividual, skos:Concept ;
	rdfs:isDefinedBy ods: ;
	rdfs:label "On deny"@en ;
	skos:definition "Log usage information or notify a party when performing the action of the rule is prohibited."@en ;
    skos:scopeNote "Non-Normative"@en .

ods:onDutyExercised
	a :RightOperand, owl:NamedIndividual, skos:Concept ;
	rdfs:isDefinedBy ods: ;
	rdfs:label "On duty exercised"@en ;
	skos:definition "Log usage information or notify a party when the action of the duty is executed."@en ;
    skos:scopeNote "Non-Normative"@en .

ods:pseudonymized
	a :RightOperand, owl:NamedIndividual, skos:Concept ;
	rdfs:isDefinedBy ods: ;
	rdfs:label "Pseudonymized"@en ;
	skos:definition "Indicates that the asset is pseudonymized."@en ;
    skos:scopeNote "Non-Normative"@en .

ods:sum
	a :RightOperand, owl:NamedIndividual, skos:Concept ;
	rdfs:isDefinedBy ods: ;
	rdfs:label "Sum"@en ;
	skos:definition "The sum function to determine  the total sum of a set of numbers."@en ;
    skos:scopeNote "Non-Normative"@en .

